发现Dynamic intransitive noninterference的错误，重新写ipurge

graph_model/index.js
@@ -1,0 +1,122 @@
+
+// http://blog.thomsonreuters.com/index.php/mobile-patent-suits-graphic-of-the-day/
+var links = [{source: "Microsoft", target: "Amazon", type: "licensing"},
+             {source: "Microsoft", target: "Amazon", type: "suit"},
+             {source: "Samsung", target: "Apple", type: "suit"},
+             {source: "Microsoft", target: "Amazon", type: "resolved"}];
+//sort links by source, then target
+links.sort(function(a,b) {
+    if (a.source > b.source) {return 1;}
+    else if (a.source < b.source) {return -1;}
+    else {
+        if (a.target > b.target) {return 1;}
+        if (a.target < b.target) {return -1;}
+        else {return 0;}
+    }
+});
+//any links with duplicate source and target get an incremented 'linknum'
+for (var i=0; i<links.length; i++) {
+    if (i != 0 &&
+        links[i].source == links[i-1].source &&
+        links[i].target == links[i-1].target) {
+            links[i].linknum = links[i-1].linknum + 1;
+        }
+    else {links[i].linknum = 1;};
+};
+console.log(links)
+var nodes = {};
+
+// Compute the distinct nodes from the links.
+links.forEach(function(link) {
+  link.source = nodes[link.source] || (nodes[link.source] = {name: link.source});
+  link.target = nodes[link.target] || (nodes[link.target] = {name: link.target});
+});
+
+// nodes.push({name: "Microsoft"})
+// nodes.push({name: "Amazon"})
+// nodes.push({name: "Samsung"})
+// nodes.push({name: "Apple"})
+console.log(nodes)
+var w = 600,
+    h = 600;
+
+var force = d3.layout.force()
+    .nodes(d3.values(nodes))
+    .links(links)
+    .size([w, h])
+    .linkDistance(60)
+    .charge(-300)
+    .on("tick", tick)
+    .start();
+
+console.log(force.nodes())
+
+var svg = d3.select("body").append("svg:svg")
+    .attr("width", w)
+    .attr("height", h);
+
+// Per-type markers, as they don't inherit styles.
+svg.append("svg:defs").selectAll("marker")
+    .data(["suit", "licensing", "resolved"])
+  .enter().append("svg:marker")
+    .attr("id", String)
+    .attr("viewBox", "0 -5 10 10")
+    .attr("refX", 15)
+    .attr("refY", -1.5)
+    .attr("markerWidth", 6)
+    .attr("markerHeight", 6)
+    .attr("orient", "auto")
+  .append("svg:path")
+    .attr("d", "M0,-5L10,0L0,5");
+
+var path = svg.append("svg:g").selectAll("path")
+    .data(force.links())
+  .enter().append("svg:path")
+    .attr("class", function(d) { return "link " + d.type; })
+    .attr("marker-end", function(d) { return "url(#" + d.type + ")"; });
+
+var circle = svg.append("svg:g").selectAll("circle")
+    .data(force.nodes().slice(0,2))
+  .enter().append("svg:circle")
+    .attr("r", 9)
+    .call(force.drag);
+
+circle = svg.append("svg:g").selectAll("circle")
+    .data(force.nodes().slice(2,4))
+  .enter().append("svg:circle")
+    .attr("r", 6)
+    .call(force.drag);
+
+var text = svg.append("svg:g").selectAll("g")
+    .data(force.nodes())
+  .enter().append("svg:g");
+
+// A copy of the text with a thick white stroke for legibility.
+text.append("svg:text")
+    .attr("x", 8)
+    .attr("y", ".31em")
+    .attr("class", "shadow")
+    .text(function(d) { return d.name; });
+
+text.append("svg:text")
+    .attr("x", 8)
+    .attr("y", ".31em")
+    .text(function(d) { return d.name; });
+
+// Use elliptical arc path segments to doubly-encode directionality.
+function tick() {
+  path.attr("d", function(d) {
+    var dx = d.target.x - d.source.x,
+        dy = d.target.y - d.source.y,
+        dr = 75/d.linknum;  //linknum is defined above
+    return "M" + d.source.x + "," + d.source.y + "A" + dr + "," + dr + " 0 0,1 " + d.target.x + "," + d.target.y;
+  });
+
+  circle.attr("transform", function(d) {
+    return "translate(" + d.x + "," + d.y + ")";
+  });
+
+  text.attr("transform", function(d) {
+    return "translate(" + d.x + "," + d.y + ")";
+  });
+}
