System_S.thy
@@ -1,0 +1,80 @@
+theory System_S
+imports Main
+begin
+subsection {* Capability Model *}
+
+type_synonym compartment_id = nat
+type_synonym entity_id = nat
+
+datatype
+  right = Taint
+          |Endorse
+          |Grant
+          |Declassify
+          |Export
+
+record cap = 
+  target :: compartment_id
+  rights :: "right set"
+
+datatype entity = Entity "cap set"
+
+type_synonym state = "entity_id \<Rightarrow> entity option"
+
+definition diminish :: "right set \<Rightarrow> cap \<Rightarrow> cap" where
+  "diminish R cap \<equiv> cap \<lparr> rights := rights cap \<inter> R \<rparr>"
+
+definition direct_caps :: "entity \<Rightarrow> cap set"
+where
+  "direct_caps e \<equiv> case e of (Entity c) \<Rightarrow> c"
+
+definition direct_caps_of :: "state \<Rightarrow> entity_id \<Rightarrow> cap set"
+where
+  "direct_caps_of s p \<equiv>
+  case s p of
+    None \<Rightarrow> {}
+  | Some (Entity e) \<Rightarrow> e"
+
+definition cap_connected :: "state \<Rightarrow> (entity_id \<times> compartment_id) set" where
+  "cap_connected s \<equiv>{(e,comp).  \<exists>cap. cap \<in> direct_caps_of s e \<and>
+                                      target cap = comp}"
+
+definition taint_cap :: "entity_id \<Rightarrow> cap" where
+  "taint_cap e\<^sub>x \<equiv> \<lparr>target = e\<^sub>x, rights = {Taint}\<rparr>"
+
+definition endorse_cap :: "entity_id \<Rightarrow> cap" where
+  "endorse_cap e\<^sub>x \<equiv> \<lparr>target = e\<^sub>x, rights = {Endorse}\<rparr>"
+
+definition grant_cap :: "entity_id \<Rightarrow> cap" where
+  "grant_cap e\<^sub>x \<equiv> \<lparr>target = e\<^sub>x, rights = {Grant}\<rparr>"
+
+definition declassify_cap :: "entity_id \<Rightarrow> cap" where
+  "declassify_cap e\<^sub>x \<equiv> \<lparr>target = e\<^sub>x, rights = {Declassify}\<rparr>"
+
+definition export_cap :: "entity_id \<Rightarrow> cap" where
+  "export_cap e\<^sub>x \<equiv> \<lparr>target = e\<^sub>x, rights = {Export}\<rparr>"
+
+subsection {* DIFC Model *}
+
+definition taint_set :: "state \<Rightarrow> entity_id \<Rightarrow> compartment_id set" where
+  "taint_set s e \<equiv> {comp. \<forall>cap. cap \<in> direct_caps_of s e \<and> Taint \<in> rights cap}"
+
+definition taint_dominate :: "state \<Rightarrow> entity_id \<Rightarrow> entity_id \<Rightarrow> bool" where
+  "taint_dominate s e\<^sub>x e\<^sub>y \<equiv>( taint_set s e\<^sub>x \<subseteq> taint_set s e\<^sub>y )"
+
+definition can_send :: "state \<Rightarrow> entity_id \<Rightarrow> entity_id \<Rightarrow> bool" where
+  "can_send s e\<^sub>x e\<^sub>y \<equiv> ( taint_set s e\<^sub>x \<subseteq> taint_set s e\<^sub>y )"
+
+definition can_declassfy_send :: "state \<Rightarrow> entity_id \<Rightarrow> entity_id \<Rightarrow> cap \<Rightarrow> bool"
+  where
+        "can_declassfy_send s e_src e_dst declassfy_cap \<equiv>
+            (declassfy_cap \<in> direct_caps_of s e_src 
+              \<and> taint_set s e_src - {target declassfy_cap} \<subseteq> taint_set s e_dst )"
+                                         
+definition can_export_send :: "state \<Rightarrow> entity_id \<Rightarrow> entity_id \<Rightarrow> cap \<Rightarrow> bool"
+  where
+        "can_export_send s e_src e_dst export_cap_s \<equiv>
+            (export_cap_s \<in> direct_caps_of s e_src 
+              \<and> taint_set s e_src \<union> {target export_cap_s} \<subseteq> taint_set s e_dst )"
+
+end
