TraditionalDIFC.thy
@@ -1,0 +1,295 @@
+theory TraditionalDIFC
+imports DynamicSecurityModel
+begin
+subsection {* Definitions *}
+
+typedecl Message
+type_synonym tag_id = nat
+datatype tag_type = SECRECY | INTEGRITY
+record tag =           
+  id :: tag_id
+  type :: tag_type   
+
+type_synonym domain_id = nat
+type_synonym domain_name = string
+
+datatype
+  right = TAG_ADD
+          |TAG_REMOVE
+
+record cap = 
+  target :: tag_id
+  rights :: "right set"     
+                            
+record label = 
+  tags :: "tag set"
+
+record domain = 
+  id_of_domain :: domain_id
+  label_of_domain :: label
+  cap_config :: "cap set"
+
+datatype Domain_Conf = DomainConf domain_id domain_name
+                           
+type_synonym Domains = "domain_id \<rightharpoonup> Domain_Conf"
+
+record State = 
+  domains :: "domain set"
+  next_tag_id :: tag_id
+
+record Sys_Config = 
+  domain_conf :: Domains
+
+consts sysconf :: "Sys_Config" 
+
+definition system_init :: "Sys_Config \<Rightarrow> State"
+  where "system_init sc \<equiv> \<lparr>domains = {},
+                           next_tag_id = 0\<rparr>"
+
+subsection {* Events *}
+
+datatype Event = Create_Tag domain_id tag_type
+                   |Change_Label domain_id tag_type label
+                   |Get_Label domain_id
+                   |Get_Caps domain_id
+                   |Send_Message domain_id domain_id Message
+
+definition domain_id_is_valid :: "State \<Rightarrow> domain_id \<Rightarrow> bool" where
+  "domain_id_is_valid s domain_id  \<equiv>
+          (if (\<exists>d. d \<in> (domains s) \<and> id_of_domain d = domain_id )
+          then True
+          else False)
+          "
+
+definition get_domain :: "State \<Rightarrow> domain_id \<Rightarrow> domain option" where
+  "get_domain s domain_id  \<equiv>
+          (if (\<exists>d. d \<in> (domains s) \<and> id_of_domain d = domain_id )
+          then Some (SOME d. d \<in> (domains s) \<and> id_of_domain d = domain_id)
+          else None)   
+          "
+
+definition get_domain2 :: "State \<Rightarrow> domain_id \<Rightarrow> (State \<times> domain option)" where
+  "get_domain2 s domain_id  \<equiv>
+          (if (\<exists>d. d \<in> (domains s) \<and> id_of_domain d = domain_id )
+          then (s, get_domain s domain_id)
+          else (s, None)               
+          )"
+
+definition get_label_by_domain_id :: "State \<Rightarrow> domain_id \<Rightarrow> label option " where
+  "get_label_by_domain_id s domain_id  \<equiv>
+            (if ((get_domain s domain_id) \<noteq> None )
+            then Some (SOME lb. \<exists>d. d \<in> (domains s) \<and> id_of_domain d = domain_id \<and> lb = label_of_domain d)
+            else None   
+            )"
+
+definition get_secrecy_label_by_domain_id :: "State \<Rightarrow> domain_id \<Rightarrow> label option " where
+  "get_secrecy_label_by_domain_id s d_id  \<equiv>
+            (if ((get_domain s d_id) \<noteq> None )
+            then 
+              let
+                dom = the (get_domain s d_id);
+                lbl = label_of_domain dom;
+                tag_set = tags lbl
+              in
+                Some (\<lparr>tags = {tg. tg \<in> tag_set \<and> type tg = SECRECY}\<rparr>)
+            else None   
+            )"
+
+definition get_integrity_label_by_domain_id :: "State \<Rightarrow> domain_id \<Rightarrow> label option " where
+  "get_integrity_label_by_domain_id s d_id  \<equiv>
+            (if ((get_domain s d_id) \<noteq> None )
+            then 
+              let
+                dom = the (get_domain s d_id);
+                lbl = label_of_domain dom;
+                tag_set = tags lbl
+              in
+                Some (\<lparr>tags = {tg. tg \<in> tag_set \<and> type tg = INTEGRITY}\<rparr>)
+            else None   
+            )"
+
+definition get_label :: "State \<Rightarrow> domain_id \<Rightarrow> (State \<times> label option) " where
+  "get_label s domain_id \<equiv>
+          (if (\<exists>d. d \<in> (domains s) \<and> id_of_domain d = domain_id )
+          then (s, get_label_by_domain_id s domain_id )
+          else (s, None)                             
+          )"
+
+definition get_caps_by_domain_id :: "State \<Rightarrow> domain_id \<Rightarrow> cap set option " where
+  "get_caps_by_domain_id s domain_id  \<equiv>
+            (if ((get_domain s domain_id) \<noteq> None )
+            then Some (SOME cap_s. \<exists>d. d \<in> (domains s) \<and> id_of_domain d = domain_id \<and> cap_s = cap_config d)
+            else None                   
+            )"
+
+definition get_add_caps_from :: "cap set \<Rightarrow> cap set" where
+  "get_add_caps_from cs \<equiv> {c. c \<in> cs \<and> TAG_ADD \<in> rights c}"
+
+definition get_addable_tag_ids_from :: "cap set \<Rightarrow> tag_id set" where
+  "get_addable_tag_ids_from cs \<equiv> {t. \<exists>c. c \<in> cs \<and> TAG_ADD \<in> rights c \<and> t = target c }"
+
+definition get_removable_tag_ids_from :: "cap set \<Rightarrow> tag_id set" where
+  "get_removable_tag_ids_from cs \<equiv> {t. \<exists>c. c \<in> cs \<and> TAG_REMOVE \<in> rights c \<and> t = target c }"
+
+definition get_caps :: "State \<Rightarrow> domain_id \<Rightarrow> (State \<times> (cap set) option) " where
+  "get_caps s domain_id \<equiv>
+          (if (\<exists>d. d \<in> (domains s) \<and> id_of_domain d = domain_id )
+          then (s, Some (SOME lb. \<exists>d. d \<in> (domains s) \<and> id_of_domain d = domain_id \<and> lb = cap_config d))
+          else (s, None)                             
+          )"
+
+definition create_tag_add_new_caps_to_domain :: "domain \<Rightarrow> cap set \<Rightarrow> domain" where
+  "create_tag_add_new_caps_to_domain d cs \<equiv> 
+          \<lparr> id_of_domain = id_of_domain d,
+            label_of_domain = label_of_domain d,
+            cap_config = cs \<union> (cap_config d)\<rparr>"
+
+
+definition create_tag_add_new_caps_to_domain_1 :: "State \<Rightarrow> domain_id \<Rightarrow> cap set \<Rightarrow> domain" where
+  "create_tag_add_new_caps_to_domain_1 s d_id cs \<equiv> 
+          let d = the (get_domain s d_id)
+          in
+          \<lparr> id_of_domain = id_of_domain d,
+            label_of_domain = label_of_domain d,
+            cap_config = cs \<union> (cap_config d)\<rparr>"
+
+definition create_tag_state_trans :: "State \<Rightarrow> domain_id \<Rightarrow> tag \<Rightarrow> State" where
+  "create_tag_state_trans s d_id tag_1 \<equiv> 
+          let rest_domains = {v. v\<in>domains s \<and> \<not> (id_of_domain v = d_id) };
+              new_add_cap =  \<lparr> target = id tag_1,
+                             rights = {TAG_ADD, TAG_REMOVE} \<rparr>;
+              new_domain = create_tag_add_new_caps_to_domain_1 s d_id {new_add_cap}
+          in
+           \<lparr> domains = insert new_domain rest_domains,
+             next_tag_id = next_tag_id s + 1 \<rparr>"
+
+definition create_tag :: "State \<Rightarrow> domain_id \<Rightarrow> tag_type \<Rightarrow> (State \<times> tag option) " where
+  "create_tag s domain_id tt \<equiv>
+          if((tt = SECRECY \<or> tt = INTEGRITY) \<and> domain_id_is_valid s domain_id )
+          then
+            let newTag = \<lparr> id = next_tag_id s,
+                          type = SECRECY \<rparr>;
+                target_domain = get_domain s domain_id
+            in (create_tag_state_trans s domain_id newTag, Some newTag)
+          else
+            (s, None)
+          "
+(*Change_Label domain_id tag_type label*)
+
+definition is_domain_label_changable :: "State \<Rightarrow> domain_id \<Rightarrow> tag_type \<Rightarrow> label \<Rightarrow> bool"
+  where
+  "is_domain_label_changable s d_id tt lbl \<equiv>
+          let cur_lbl = (the (get_label_by_domain_id s d_id));
+              cur_cap_set = (the (get_caps_by_domain_id s d_id));
+              cur_addable_tag_ids = get_addable_tag_ids_from cur_cap_set;
+              cur_removable_tag_ids = get_removable_tag_ids_from cur_cap_set
+          in
+          if (tt = SECRECY \<or> tt = INTEGRITY)
+          then
+            if((\<forall>t. t\<in>tags lbl
+                   \<and> \<not> (t\<in>tags cur_lbl)
+                   \<and> (id t)\<in> cur_addable_tag_ids)
+                \<or>
+                (\<forall>t. \<not>(t\<in>tags lbl)
+                   \<and> t\<in>tags cur_lbl
+                   \<and> (id t)\<in> cur_addable_tag_ids))
+            then
+              True
+            else
+              False
+          else
+            False
+  "
+
+definition change_label_of_domain :: "State \<Rightarrow> domain_id \<Rightarrow> label \<Rightarrow> domain" where
+  "change_label_of_domain s d_id lbl \<equiv> 
+          let d = the (get_domain s d_id)         
+          in
+          \<lparr> id_of_domain = id_of_domain d,
+            label_of_domain = lbl,
+            cap_config = cap_config d\<rparr>"
+
+
+definition change_label_state_trans :: "State \<Rightarrow> domain_id \<Rightarrow> tag_type \<Rightarrow> label \<Rightarrow> State" where
+  "change_label_state_trans s d_id tt lbl \<equiv>
+          let rest_domains = {v. v\<in>domains s \<and> \<not> (id_of_domain v = d_id) };
+              new_domain = change_label_of_domain s d_id lbl
+          in
+           \<lparr> domains = insert new_domain rest_domains,
+             next_tag_id = next_tag_id s\<rparr>"                 
+
+definition change_label :: "State \<Rightarrow> domain_id \<Rightarrow> tag_type \<Rightarrow> label \<Rightarrow> (State \<times> bool ) " where
+  "change_label s domain_id tt lbl \<equiv>
+          if((tt = SECRECY \<or> tt = INTEGRITY)
+              \<and> domain_id_is_valid s domain_id
+              \<and> is_domain_label_changable s domain_id tt lbl)
+          then (change_label_state_trans s domain_id tt lbl, True)
+          else
+            (s, False)
+          "
+definition send_message :: "State \<Rightarrow> domain_id \<Rightarrow> domain_id \<Rightarrow> Message \<Rightarrow> State"
+  where
+  "send_message s src_id dst_id m \<equiv>
+        s
+        "
+                                                
+definition exec_event :: "State \<Rightarrow> Event \<Rightarrow> State" where
+  "exec_event s e  \<equiv>
+    case e of  Create_Tag d_id tt \<Rightarrow> fst (create_tag s d_id tt)
+               |Change_Label d_id tt lbl \<Rightarrow> fst (change_label s d_id tt lbl )
+               |Get_Label d_id \<Rightarrow> fst (get_label s d_id)
+               |Get_Caps d_id \<Rightarrow> fst (get_caps s d_id)
+               |Send_Message src_id dst_id msg \<Rightarrow> s
+               "
+(*
+definition dominates :: "label \<Rightarrow> label \<Rightarrow> bool"
+*)
+
+definition domain_of_event :: "Event \<Rightarrow> domain_id option"
+  where
+    "domain_of_event e \<equiv> 
+          case e of  Create_Tag d_id tt \<Rightarrow> Some d_id
+               |Change_Label d_id tt lbl \<Rightarrow> Some d_id
+               |Get_Label d_id \<Rightarrow> Some d_id
+               |Get_Caps d_id \<Rightarrow> Some d_id
+               |Send_Message src_id dst_id msg \<Rightarrow> Some src_id
+               "
+
+definition interference1 :: "domain_id \<Rightarrow> State \<Rightarrow> domain_id \<Rightarrow> bool" ("(_ \<leadsto> _)")
+    where                                                                                                  
+      "interference1 d1 s d2 \<equiv>
+          let
+            secrecy_lbl1 = the (get_secrecy_label_by_domain_id s d1);
+            secrecy_lbl2 = the (get_secrecy_label_by_domain_id s d2);
+            integrity_lbl1 = the (get_integrity_label_by_domain_id s d1);
+            integrity_lbl2 = the (get_integrity_label_by_domain_id s d2)
+          in
+          if d1 = d2 then True
+          else if d1 \<noteq> d2
+            then
+              tags secrecy_lbl1 \<subseteq> tags secrecy_lbl2 \<and> 
+              tags integrity_lbl1 \<subseteq> tags integrity_lbl2
+          else False"             
+
+definition vpeq1 :: "State \<Rightarrow> domain_id \<Rightarrow> State \<Rightarrow> bool"
+  where
+    "vpeq1 s d t \<equiv> 
+        let
+          d1 = get_domain s d;
+          d2 = get_domain t d
+        in
+          if(d1 = d2)
+          then
+            True
+          else
+            False
+          "
+
+consts s0t :: State
+definition s0t_witness :: State
+  where "s0t_witness \<equiv> system_init sysconf"
+specification (s0t) 
+  s0t_init: "s0t = system_init sysconf"
+  by simp
+
+end
